examples/hoare_logic/blocking_semantics3/blocking_semantics3_WP_progress_1.v
@@ -4,7 +4,6 @@ Require Import BuiltIn.
 Require BuiltIn.
 Require int.Int.
 Require int.MinMax.
-Require set.Set.
 
 (* Why3 assumption *)
 Inductive list (a:Type) {a_WT:WhyType a} :=
@@ -576,32 +575,109 @@ Definition total_valid_triple(p:fmla) (s:stmt) (q:fmla): Prop :=
   exists pi':(list (ident* value)%type), exists n:Z, (many_steps sigma pi s
   sigma' pi' Sskip n) /\ (eval_fmla sigma' pi' q).
 
-(* Why3 assumption *)
-Definition assigns(sigma:(map mident value)) (a:(set.Set.set mident))
-  (sigma':(map mident value)): Prop := forall (i:mident), (~ (set.Set.mem i
-  a)) -> ((get sigma i) = (get sigma' i)).
+Axiom set1 : forall (a:Type) {a_WT:WhyType a}, Type.
+Parameter set1_WhyType : forall (a:Type) {a_WT:WhyType a}, WhyType (set1 a).
+Existing Instance set1_WhyType.
 
-Axiom assigns_refl : forall (sigma:(map mident value)) (a:(set.Set.set
-  mident)), (assigns sigma a sigma).
+Parameter mem1: forall {a:Type} {a_WT:WhyType a}, a -> (set1 a) -> Prop.
+
+(* Why3 assumption *)
+Definition infix_eqeq {a:Type} {a_WT:WhyType a}(s1:(set1 a)) (s2:(set1
+  a)): Prop := forall (x:a), (mem1 x s1) <-> (mem1 x s2).
+
+Axiom extensionality : forall {a:Type} {a_WT:WhyType a}, forall (s1:(set1 a))
+  (s2:(set1 a)), (infix_eqeq s1 s2) -> (s1 = s2).
+
+(* Why3 assumption *)
+Definition subset {a:Type} {a_WT:WhyType a}(s1:(set1 a)) (s2:(set1
+  a)): Prop := forall (x:a), (mem1 x s1) -> (mem1 x s2).
+
+Axiom subset_trans : forall {a:Type} {a_WT:WhyType a}, forall (s1:(set1 a))
+  (s2:(set1 a)) (s3:(set1 a)), (subset s1 s2) -> ((subset s2 s3) ->
+  (subset s1 s3)).
+
+Parameter empty: forall {a:Type} {a_WT:WhyType a}, (set1 a).
+
+(* Why3 assumption *)
+Definition is_empty {a:Type} {a_WT:WhyType a}(s:(set1 a)): Prop :=
+  forall (x:a), ~ (mem1 x s).
+
+Axiom empty_def1 : forall {a:Type} {a_WT:WhyType a}, (is_empty (empty :(set1
+  a))).
+
+Parameter add: forall {a:Type} {a_WT:WhyType a}, a -> (set1 a) -> (set1 a).
+
+Axiom add_def1 : forall {a:Type} {a_WT:WhyType a}, forall (x:a) (y:a),
+  forall (s:(set1 a)), (mem1 x (add y s)) <-> ((x = y) \/ (mem1 x s)).
+
+Parameter remove: forall {a:Type} {a_WT:WhyType a}, a -> (set1 a) -> (set1
+  a).
+
+Axiom remove_def1 : forall {a:Type} {a_WT:WhyType a}, forall (x:a) (y:a)
+  (s:(set1 a)), (mem1 x (remove y s)) <-> ((~ (x = y)) /\ (mem1 x s)).
+
+Axiom subset_remove : forall {a:Type} {a_WT:WhyType a}, forall (x:a) (s:(set1
+  a)), (subset (remove x s) s).
+
+Parameter union: forall {a:Type} {a_WT:WhyType a}, (set1 a) -> (set1 a) ->
+  (set1 a).
+
+Axiom union_def1 : forall {a:Type} {a_WT:WhyType a}, forall (s1:(set1 a))
+  (s2:(set1 a)) (x:a), (mem1 x (union s1 s2)) <-> ((mem1 x s1) \/ (mem1 x
+  s2)).
+
+Parameter inter: forall {a:Type} {a_WT:WhyType a}, (set1 a) -> (set1 a) ->
+  (set1 a).
+
+Axiom inter_def1 : forall {a:Type} {a_WT:WhyType a}, forall (s1:(set1 a))
+  (s2:(set1 a)) (x:a), (mem1 x (inter s1 s2)) <-> ((mem1 x s1) /\ (mem1 x
+  s2)).
+
+Parameter diff: forall {a:Type} {a_WT:WhyType a}, (set1 a) -> (set1 a) ->
+  (set1 a).
+
+Axiom diff_def1 : forall {a:Type} {a_WT:WhyType a}, forall (s1:(set1 a))
+  (s2:(set1 a)) (x:a), (mem1 x (diff s1 s2)) <-> ((mem1 x s1) /\ ~ (mem1 x
+  s2)).
+
+Axiom subset_diff : forall {a:Type} {a_WT:WhyType a}, forall (s1:(set1 a))
+  (s2:(set1 a)), (subset (diff s1 s2) s1).
+
+Parameter choose: forall {a:Type} {a_WT:WhyType a}, (set1 a) -> a.
+
+Axiom choose_def : forall {a:Type} {a_WT:WhyType a}, forall (s:(set1 a)),
+  (~ (is_empty s)) -> (mem1 (choose s) s).
+
+Parameter all: forall {a:Type} {a_WT:WhyType a}, (set1 a).
+
+Axiom all_def : forall {a:Type} {a_WT:WhyType a}, forall (x:a), (mem1 x
+  (all :(set1 a))).
+
+(* Why3 assumption *)
+Definition assigns(sigma:(map mident value)) (a:(set1 mident)) (sigma':(map
+  mident value)): Prop := forall (i:mident), (~ (mem1 i a)) -> ((get sigma
+  i) = (get sigma' i)).
+
+Axiom assigns_refl : forall (sigma:(map mident value)) (a:(set1 mident)),
+  (assigns sigma a sigma).
 
 Axiom assigns_trans : forall (sigma1:(map mident value)) (sigma2:(map mident
-  value)) (sigma3:(map mident value)) (a:(set.Set.set mident)),
-  ((assigns sigma1 a sigma2) /\ (assigns sigma2 a sigma3)) -> (assigns sigma1
-  a sigma3).
+  value)) (sigma3:(map mident value)) (a:(set1 mident)), ((assigns sigma1 a
+  sigma2) /\ (assigns sigma2 a sigma3)) -> (assigns sigma1 a sigma3).
 
 Axiom assigns_union_left : forall (sigma:(map mident value)) (sigma':(map
-  mident value)) (s1:(set.Set.set mident)) (s2:(set.Set.set mident)),
-  (assigns sigma s1 sigma') -> (assigns sigma (set.Set.union s1 s2) sigma').
+  mident value)) (s1:(set1 mident)) (s2:(set1 mident)), (assigns sigma s1
+  sigma') -> (assigns sigma (union s1 s2) sigma').
 
 Axiom assigns_union_right : forall (sigma:(map mident value)) (sigma':(map
-  mident value)) (s1:(set.Set.set mident)) (s2:(set.Set.set mident)),
-  (assigns sigma s2 sigma') -> (assigns sigma (set.Set.union s1 s2) sigma').
+  mident value)) (s1:(set1 mident)) (s2:(set1 mident)), (assigns sigma s2
+  sigma') -> (assigns sigma (union s1 s2) sigma').
 
 (* Why3 assumption *)
-Fixpoint stmt_writes(s:stmt) (w:(set.Set.set mident)) {struct s}: Prop :=
+Fixpoint stmt_writes(s:stmt) (w:(set1 mident)) {struct s}: Prop :=
   match s with
   | (Sskip|(Sassert _)) => True
-  | (Sassign id _) => (set.Set.mem id w)
+  | (Sassign id _) => (mem1 id w)
   | (Sseq s1 s2) => (stmt_writes s1 w) /\ (stmt_writes s2 w)
   | (Sif t s1 s2) => (stmt_writes s1 w) /\ (stmt_writes s2 w)
   | (Swhile _ _ body) => (stmt_writes body w)
@@ -617,10 +693,16 @@ Axiom abstract_effects_generalize : forall (sigma:(map mident value))
   (pi:(list (ident* value)%type)) (s:stmt) (f:fmla), (eval_fmla sigma pi
   (abstract_effects s f)) -> (eval_fmla sigma pi f).
 
-Axiom abstract_effects_monotonic : forall (s:stmt) (f:fmla),
-  forall (sigma:(map mident value)) (pi:(list (ident* value)%type)),
-  (eval_fmla sigma pi f) -> forall (sigma1:(map mident value)) (pi1:(list
-  (ident* value)%type)), (eval_fmla sigma1 pi1 (abstract_effects s f)).
+Axiom abstract_effects_distrib_conj : forall (s:stmt) (p:fmla) (q:fmla)
+  (sigma:(map mident value)) (pi:(list (ident* value)%type)),
+  ((eval_fmla sigma pi (abstract_effects s p)) /\ (eval_fmla sigma pi
+  (abstract_effects s q))) -> (eval_fmla sigma pi (abstract_effects s (Fand p
+  q))).
+
+Axiom abstract_effects_monotonic : forall (s:stmt) (p:fmla) (q:fmla),
+  (valid_fmla (Fimplies p q)) -> forall (sigma:(map mident value)) (pi:(list
+  (ident* value)%type)), (eval_fmla sigma pi (abstract_effects s p)) ->
+  (eval_fmla sigma pi (abstract_effects s q)).
 
 (* Why3 assumption *)
 Fixpoint wp(s:stmt) (q:fmla) {struct s}: fmla :=
@@ -678,3 +760,4 @@ do 3 eexists.
 econstructor.
 eauto.
 Qed.
+
